Fix Delayed.v

src/sequential/Delayed.v
@@ -34,20 +34,11 @@ Require Import gSimAux.
 
 Set Implicit Arguments.
 
-Inductive joined_promise_steps lang:
-  forall (th0 th1: Thread.t lang) (views0 views1: Loc.t -> Time.t -> list View.t), Prop :=
-| joined_promise_steps_base
-    th0 views0
-  :
-    joined_promise_steps th0 th0 views0 views0
-| joined_promise_steps_step
-    th0 th1 th2 views0 views1 views2
-    pf loc from to msg kind
-    (STEP: JThread.step pf (ThreadEvent.promise loc from to msg kind) th0 th1 views0 views1)
-    (STEPS: joined_promise_steps th1 th2 views1 views2)
-  :
-    joined_promise_steps th0 th2 views0 views2
-.
+Definition is_promise (e: ThreadEvent.t): Prop :=
+  match e with
+  | ThreadEvent.promise _ _ _ _ _ => True
+  | _ => False
+  end.
 
 Definition release_event (e: ThreadEvent.t): Prop :=
   match e with
@@ -61,9 +52,9 @@ Definition release_event (e: ThreadEvent.t): Prop :=
   | _ => False
   end.
 
-Variant lower_step views {lang} e (th0 th1: Thread.t lang): Prop :=
+Variant lower_step {lang} e (th0 th1: Thread.t lang): Prop :=
 | lower_step_intro
-    (STEP: JThread.step true e th0 th1 views views)
+    (STEP: Thread.step true e th0 th1)
     (NPROMISE: no_promise e)
     (NRELEASE: ~ release_event e)
     (MEM: lower_memory th1.(Thread.memory) th0.(Thread.memory))
@@ -84,26 +75,20 @@ Proof.
     hexploit lower_memory_get; eauto. i. des; clarify. }
 Qed.
 
-Lemma step_split_pure lang (th0 th2: Thread.t lang) e views0 views2
-      (STEP: JThread.step true e th0 th2 views0 views2)
+Lemma step_split_pure lang (th0 th2: Thread.t lang) e
+      (STEP: Thread.step true e th0 th2)
       (NPROMISE: no_promise e)
       (NRELEASE: ~ release_event e)
       (MEM: th2.(Thread.memory) = th0.(Thread.memory))
   :
     exists th1,
-      (<<PROMISES: joined_promise_steps th0 th1 views0 views2>>) /\
-      (<<LOWER: rtc (tau (lower_step views2)) th1 th2>>) /\
+      (<<PROMISES: rtc (tau (@pred_step is_promise _)) th0 th1>>) /\
+      (<<LOWER: rtc (tau lower_step) th1 th2>>) /\
       (<<MEM: th1.(Thread.memory) = th2.(Thread.memory)>>) /\
       (<<SC: th1.(Thread.sc) = th2.(Thread.sc)>>).
 Proof.
-  inv STEP. assert (views2 = views0).
-  { extensionality loc. extensionality ts.
-    destruct (classic (views2 loc ts = views0 loc ts)); auto.
-    hexploit VIEWSLE; eauto. i. des.
-    rewrite MEM in *. clarify.
-  }
   assert (SC: th2.(Thread.sc) = th0.(Thread.sc)).
-  { inv STEP0; inv STEP; auto. inv LOCAL; ss.
+  { inv STEP; inv STEP0; auto. inv LOCAL; ss.
     { inv LOCAL0; ss. }
     { inv LOCAL1; inv LOCAL2; ss. }
     { inv LOCAL0; ss.
@@ -160,110 +145,110 @@ Proof.
     left. esplits; eauto. refl. }
 Qed.
 
-Definition views_mem_le
-           (mem0 mem1: Memory.t)
-           (views0 views1: Loc.t -> Time.t -> list View.t)
-           (tvw: TView.t): Prop :=
-  forall loc ts (NEQ: views1 loc ts <> views0 loc ts),
-    (<<NIL: views0 loc ts = []>>) /\
-    exists from val released,
-      (<<GET: Memory.get loc ts mem1 = Some (from, Message.concrete val (Some released))>>) /\
-      (<<NONE: Memory.get loc ts mem0 = None>>) /\
-      (<<VIEW: views1 loc ts = (View.join (tvw.(TView.rel) loc) (View.singleton_ur loc ts))
-                                 ::(all_join_views (View.singleton_ur loc ts) (views0 loc from))>>).
-
-Lemma write_tview_join_singleton tvw sc loc0 ts0 ord loc1 ts1
-      (ORD: ~ Ordering.le Ordering.acqrel ord)
-      (TS: loc0 = loc1 -> Time.le ts0 ts1)
+Lemma promise_step_tau_promise_step lang (th0 th1: Thread.t lang)
+      pf e
+      (STEP: Thread.promise_step pf e th0 th1)
   :
-    View.join (TView.rel (TView.write_tview tvw sc loc0 ts0 ord) loc1)
-              (View.singleton_ur loc1 ts1) =
-    View.join (TView.rel tvw loc1) (View.singleton_ur loc1 ts1).
+    tau (@pred_step is_promise _) th0 th1.
 Proof.
-  ss. des_ifs. setoid_rewrite LocFun.add_spec; eauto.
-  destruct (LocSet.Facts.eq_dec loc1 loc0).
-  { subst. rewrite View.join_assoc. f_equal.
-    rewrite singleton_ur_join. f_equal.
-    apply TimeFacts.le_join_r. auto. }
-  { refl. }
+  econs; eauto.
+  { econs; eauto.
+    { econs; eauto. econs 1; eauto. }
+    { inv STEP; ss. }
+  }
+  { inv STEP; ss. }
 Qed.
 
-Local Opaque TView.write_tview.
+Lemma lower_step_tau_lower_step lang (th0 th1: Thread.t lang)
+      e
+      (STEP: lower_step e th0 th1)
+  :
+    tau lower_step th0 th1.
+Proof.
+  inv STEP. econs; eauto.
+  { econs; eauto. }
+  { destruct e; ss. }
+Qed.
 
-Lemma step_split lang (th0 th2: Thread.t lang) pf e views0 views2
-      (STEP: JThread.step pf e th0 th2 views0 views2)
+Lemma memory_lower_exists
+      prom0 mem0 loc from to msg
+      (CLOSED: Memory.closed mem0)
+      (MLE: Memory.le prom0 mem0)
+      (MSG: msg <> Message.reserve)
+      (GET: Memory.get loc to prom0 = Some (from, msg))
+      (BOT: Memory.bot_none prom0)
+  :
+    Memory.promise prom0 mem0 loc from to msg prom0 mem0 (Memory.op_kind_lower msg).
+Proof.
+  inv CLOSED. exploit CLOSED0.
+  { eapply MLE. eauto. }
+  i. des.
+  hexploit Memory.lower_exists; try eassumption.
+  { hexploit memory_get_ts_strong; eauto. i. des; clarify.
+    rewrite BOT in GET. ss. }
+  { refl. }
+  i. des. hexploit Memory.lower_exists_le; eauto. i. des.
+  hexploit lower_same_same; try apply H. i. subst.
+  hexploit lower_same_same; try apply H0. i. subst.
+  econs; eauto.
+Qed.
+
+Lemma step_split lang (th0 th2: Thread.t lang) pf e
+      (STEP: Thread.step pf e th0 th2)
       (NRELEASE: ~ release_event e)
       (LOCAL: Local.wf (Thread.local th0) (Thread.memory th0))
       (SC: Memory.closed_timemap (Thread.sc th0) (Thread.memory th0))
       (CLOSED: Memory.closed (Thread.memory th0))
       (CONS: Local.promise_consistent th2.(Thread.local))
-      (MEMORY: joined_memory views0 th0.(Thread.memory))
-      (VIEWS: wf_views views0)
-      (RELEASED: joined_released views0 th0.(Thread.local).(Local.promises) th0.(Thread.local).(Local.tview).(TView.rel))
   :
     exists th1,
-      (<<PROMISES: joined_promise_steps th0 th1 views0 views2>>) /\
-      (<<LOWER: rtc (tau (lower_step views2)) th1 th2>>) /\
+      (<<PROMISES: rtc (tau (@pred_step is_promise _)) th0 th1>>) /\
+      (<<LOWER: rtc (tau lower_step) th1 th2>>) /\
       (<<MEM: th1.(Thread.memory) = th2.(Thread.memory)>>) /\
       (<<SC: th1.(Thread.sc) = th2.(Thread.sc)>>).
 Proof.
+  hexploit Thread.step_future; eauto. i. des.
   dup STEP. inv STEP.
-  assert (VIEWSLE0: views_le views0 views2).
-  { ii. apply NNPP. ii. hexploit VIEWSLE; eauto. i. des; ss. }
-  inv STEP1.
-  { inv STEP. esplits.
-    { econs; [|econs]. econs; eauto.
-      { econs. econs; eauto. }
+  { exists th2. inv STEP1. ss. splits; eauto.
+    econs; eauto. econs.
+    { econs; eauto.
+      { econs; eauto. }
+      { ss. }
     }
-    { econs. }
-    { ss. }
     { ss. }
   }
-  { inv STEP. inv LOCAL0; ss.
+  { inv STEP1. inv LOCAL0; ss.
     { eapply step_split_pure; eauto; ss. }
     { eapply step_split_pure; eauto; ss. }
     { inv LOCAL1. ss. dup WRITE. inv WRITE. esplits.
-      { econs; [|econs]. econs.
-        { econs. econs; ss. econs.
+      { econs; [|econs]. eapply promise_step_tau_promise_step.
+        econs.
+        { econs; eauto. econs; ss. eapply TViewFacts.op_closed_released.
+          { eapply SC. }
           { eauto. }
-          { econs; ss. eapply TViewFacts.op_closed_released; eauto.
-            { eapply LOCAL. }
-            { eapply Memory.write_op; eauto. }
+          { eapply LOCAL. }
+          { eauto. }
+          { eapply Memory.write_op; eauto. }
+        }
+        { ss. }
+      }
+      { econs; [|econs]. eapply lower_step_tau_lower_step.
+        { econs.
+          { econs 2. econs; eauto; cycle 1.
+            { econs 3. econs; eauto; ss. econs; eauto.
+              eapply memory_lower_exists; eauto.
+              { eapply promise_memory_le; eauto. eapply LOCAL. }
+              { ss. }
+              { eapply Memory.remove_get0 in REMOVE. des. auto. }
+              { eapply Memory.promise_bot_none; eauto. eapply LOCAL. }
+            }
+            { ss. }
           }
           { ss. }
-        }
-        { i. clarify. unfold TView.write_released in *.
-          destruct (Ordering.le Ordering.relaxed ord) eqn:ORD0; econs.
-          inv MEMORY0. hexploit (COMPLETE loc0 to0).
-          { eapply Memory.write_get2 in WRITE0. des; eauto. }
-          rewrite View.join_bot_l. ss.
-          replace (Ordering.le Ordering.acqrel ord) with false in *.
-          2:{ destruct ord; ss. }
-          i. des. auto.
-        }
-        { i. ss.
-          hexploit VIEWSLE; eauto. i. des.
-          assert (ts = to).
-          { eapply Memory.promise_op in PROMISE0.
-            eapply memory_op_diff_only in PROMISE0; eauto. des; clarify. }
-          subst. esplits; eauto.
-          rewrite write_tview_join_singleton in VIEW; eauto.
-          { destruct ord; ss. }
-          { i. refl. }
-        }
-        { auto. }
-        { auto. }
-        { ss. ii. eapply Memory.promise_op_promise in PROMISE0. dup GET.
-          eapply memory_op_diff_only in GET0; eauto. des; clarify.
-          { inv MSG. inv RELEASED1.
-            exploit RELEASED; eauto. i.
-            replace (views0 loc0 ts) with (views2 loc0 ts) in x; auto.
-            apply NNPP. ii. exploit VIEWSLE0; eauto. ii.
-            rewrite H0 in x. ss. }
-          { admit. }
+          { ss. }
+          { ss. refl. }
         }
       }
-      { admit. }
       { ss. }
       { ss. }
     }
@@ -275,30 +260,24 @@ Proof.
 Admitted.
 
 Definition delayed {lang} (st0 st1: lang.(Language.state))
-           lc0 lc1 mem sc views fin: Prop
+           lc0 lc1 mem sc fin: Prop
   :=
     (<<MEM: Memory.closed mem>>) /\
     (<<SC: Memory.closed_timemap sc mem>>) /\
     (<<LOCAL0: Local.wf lc0 mem>>) /\
-    (<<JOINED: joined_memory views mem>>) /\
-    (<<RELEASED0: joined_released views lc0.(Local.promises) lc0.(Local.tview).(TView.rel)>>) /\
     (<<LOCAL1: Local.wf lc1 mem>>) /\
-    (<<RELEASED1: joined_released views lc1.(Local.promises) lc1.(Local.tview).(TView.rel)>>) /\
     (<<FIN: Messages.of_memory lc0.(Local.promises) <4= (Messages.of_memory lc1.(Local.promises) \4/ fin)>>) /\
     exists lc1' mem',
-      (<<STEPS: rtc (tau (lower_step views)) (Thread.mk _ st0 lc0 sc mem) (Thread.mk _ st1 lc1' sc mem')>>) /\
+      (<<STEPS: rtc (tau lower_step) (Thread.mk _ st0 lc0 sc mem) (Thread.mk _ st1 lc1' sc mem')>>) /\
       (<<MEM: lower_memory mem' mem>>) /\
       (<<LOCAL: lower_local lc1' lc1>>).
 
-Lemma delayed_refl lang (st: lang.(Language.state)) lc mem sc views fin
+Lemma delayed_refl lang (st: lang.(Language.state)) lc mem sc fin
       (MEM: Memory.closed mem)
-      (VIEWS: wf_views views)
       (SC: Memory.closed_timemap sc mem)
       (LOCAL: Local.wf lc mem)
-      (JOINED: joined_memory views mem)
-      (RELEASED: joined_released views lc.(Local.promises) lc.(Local.tview).(TView.rel))
   :
-    delayed st st lc lc mem sc views fin.
+    delayed st st lc lc mem sc fin.
 Proof.
   red. esplits; eauto.
   { refl. }
@@ -306,35 +285,32 @@ Proof.
 Qed.
 
 Lemma delayed_future
-      mem1 sc1 views1
-      lang (st0 st1: lang.(Language.state)) lc0 lc1 mem0 sc0 views0 fin0 fin1
-      (DELAYED: delayed st0 st1 lc0 lc1 mem0 sc0 views0 fin0)
+      mem1 sc1
+      lang (st0 st1: lang.(Language.state)) lc0 lc1 mem0 sc0 fin0 fin1
+      (DELAYED: delayed st0 st1 lc0 lc1 mem0 sc0 fin0)
 
       (MEM: Memory.closed mem1)
-      (VIEWS: wf_views views1)
       (SC: Memory.closed_timemap sc1 mem1)
       (LOCAL: Local.wf lc1 mem1)
       (FIN: fin1 <4= unchangable mem1 lc1.(Local.promises))
-      (JOINED: joined_memory views1 mem1)
 
       (MEM_FUTURE: Memory.future mem0 mem1)
       (SC_FUTURE: TimeMap.le sc0 sc1)
-      (VIEWS_FUTURE: views_le views0 views1)
       (FIN_FUTURE: fin0 <4= fin1)
   :
-    delayed st0 st1 lc0 lc1 mem1 sc1 views1 fin1.
+    delayed st0 st1 lc0 lc1 mem1 sc1 fin1.
 Admitted.
 
 Lemma delayed_step
       lang (st0 st1 st2: Language.state lang) lc0 lc1 lc2
-      mem1 sc1 views1 mem2 sc2 views2 fin
+      mem1 sc1 mem2 sc2 fin
       pf e
-      (STEP: JThread.step pf e (Thread.mk _ st1 lc1 sc1 mem1) (Thread.mk _ st2 lc2 sc2 mem2) views1 views2)
+      (STEP: Thread.step pf e (Thread.mk _ st1 lc1 sc1 mem1) (Thread.mk _ st2 lc2 sc2 mem2))
       (NRELEASE: ~ release_event e)
-      (DELAYED: delayed st0 st1 lc0 lc1 mem1 sc1 views1 fin)
+      (DELAYED: delayed st0 st1 lc0 lc1 mem1 sc1 fin)
   :
     exists lc0',
-      (<<PROMISES: joined_promise_steps (Thread.mk _ st0 lc0 sc1 mem1) (Thread.mk _ st0 lc0' sc2 mem2) views1 views2>>) /\
-      (<<DELAYED: delayed st0 st2 lc0' lc2 mem2 sc2 views2 (fin \4/ committed mem1 lc1.(Local.promises) mem2 lc2.(Local.promises))>>).
+      (<<PROMISES: rtc (tau (@pred_step is_promise _)) (Thread.mk _ st0 lc0 sc1 mem1) (Thread.mk _ st0 lc0' sc2 mem2)>>) /\
+      (<<DELAYED: delayed st0 st2 lc0' lc2 mem2 sc2 (fin \4/ committed mem1 lc1.(Local.promises) mem2 lc2.(Local.promises))>>).
 Proof.
 Admitted.
